Control flow break: almost done

Phi_Semantics/PhiSem_CF_Return.thy
@@ -55,18 +55,33 @@ interpretation \<phi>CF_break_fic INTERPRET FIC_brk_frame using \<phi>CF_break_f
 hide_fact \<phi>CF_break_fic_ax
 
 interpretation FIC_brk_frame:
-    identity_fiction \<open>{frames. finite (dom frames)}\<close> R_brk_frame FIC_brk_frame ..
+    identity_fiction_for_partial_mapping_resource \<open>{frames. finite (dom frames)}\<close> R_brk_frame FIC_brk_frame ..
+
 
 section \<open>\<phi>-Types\<close>
 
+(*
 abbreviation Brk_Frame' :: \<open>brk_label \<Rightarrow> (VAL list option,'a) \<phi> \<Rightarrow> (fiction,'a) \<phi>\<close>
   where \<open>Brk_Frame' label T \<equiv> (FIC_brk_frame.\<phi> (label \<^bold>\<rightarrow> \<black_circle> (Nonsepable T)))\<close>
+*)
 
-abbreviation Brk_Frame :: \<open>brk_label \<Rightarrow> assn\<close>
+definition Brk_Frame :: \<open>brk_label \<Rightarrow> assn\<close>
   where \<open>Brk_Frame label \<equiv> () \<Ztypecolon> FIC_brk_frame.\<phi> (label \<^bold>\<rightarrow> \<black_circle> (Nonsepable \<circle>))\<close>
 
-abbreviation Brking_Frame :: \<open>brk_label \<Rightarrow> (VAL list,'a) \<phi> \<Rightarrow> (fiction,'a) \<phi>\<close>
-  where \<open>Brking_Frame label T \<equiv> (FIC_brk_frame.\<phi> (label \<^bold>\<rightarrow> \<black_circle> (Nonsepable (\<black_circle> T))))\<close>
+definition Brking_Frame :: \<open>brk_label \<Rightarrow> ('v::VALs sem \<Rightarrow> assn) \<Rightarrow> assn\<close>
+  where \<open>Brking_Frame label S \<equiv>
+    (\<exists>*v. S v\<heavy_comma> to_vals (sem.dest v) \<Ztypecolon> FIC_brk_frame.\<phi> (label \<^bold>\<rightarrow> \<black_circle> (Nonsepable (\<black_circle> Identity))))\<close>
+
+lemma Brk_Frame_eq_identity:
+  \<open>Brk_Frame l = (nonsepable None \<Ztypecolon> FIC_brk_frame.\<phi> (l \<^bold>\<rightarrow> \<black_circle> Identity))\<close>
+  unfolding set_eq_iff Brk_Frame_def
+  by (simp add: \<phi>expns)
+
+lemma Brking_Frame_eq_identity:
+  \<open>Brking_Frame l S = (\<exists>*v. S v\<heavy_comma> nonsepable (Some (to_vals (sem.dest v))) \<Ztypecolon> FIC_brk_frame.\<phi> (l \<^bold>\<rightarrow> \<black_circle> Identity))\<close>
+  unfolding set_eq_iff Brking_Frame_def
+  by (simp add: \<phi>expns)
+
 
 
 section \<open>Instruction\<close>
@@ -77,82 +92,79 @@ definition op_brk_scope :: \<open>(brk_label \<Rightarrow> ('a::VALs) proc) \<Ri
     op_try
     (F l \<bind> (\<lambda>ret. R_brk_frame.\<phi>R_set_res (\<lambda>f. f(l := None)) \<ggreater> Return ret))
     (\<lambda>a. R_brk_frame.\<phi>R_get_res_entry l (\<lambda>brk.
-      case nonsepable.dest brk of Some vs \<Rightarrow> Return (sem (from_vals vs))
-                                | None \<Rightarrow> throw a
+      R_brk_frame.\<phi>R_set_res (\<lambda>f. f(l := None)) \<ggreater>
+     (case nonsepable.dest brk of Some vs \<Rightarrow> Return (sem (from_vals vs))
+                                | None \<Rightarrow> throw a)
 )))
 \<close>
 
+definition op_break :: \<open>brk_label \<Rightarrow> ('a::VALs, 'ret::VALs) proc'\<close>
+  where \<open>op_break l = (\<lambda>vs.
+     R_brk_frame.\<phi>R_set_res (\<lambda>f. f(l \<mapsto> nonsepable (Some (to_vals (sem.dest vs)))))
+  \<ggreater> throw (sem (ABN_break.mk ()))
+)\<close>
+
+
 context begin
 
-private lemma alloc:
+private lemma alloc_brk_scope[intro!]:
   \<open>(\<And>l. \<^bold>p\<^bold>r\<^bold>o\<^bold>c F l \<lbrace> X\<heavy_comma> Brk_Frame l \<longmapsto> Y \<rbrace> \<^bold>t\<^bold>h\<^bold>r\<^bold>o\<^bold>w\<^bold>s E  )
 \<Longrightarrow> \<^bold>p\<^bold>r\<^bold>o\<^bold>c R_brk_frame.\<phi>R_allocate_res_entry (\<lambda>_. True) (Some (nonsepable None)) F
          \<lbrace> X \<longmapsto> Y \<rbrace> \<^bold>t\<^bold>h\<^bold>r\<^bold>o\<^bold>w\<^bold>s E \<close>
-  apply (clarsimp simp add: \<phi>expns \<phi>Procedure_\<phi>Res_Spec simp del: set_mult_expn del: subsetI)
-  subgoal for r res c
-  apply (rule R_brk_frame.\<phi>R_allocate_res_entry[where R="(\<I> INTERP (r * c))"])
-  apply clarsimp using finite_map_freshness apply blast
-  
-  apply clarsimp
-  
-  apply (clarsimp simp del: \<phi>Res_Spec_mult_homo set_mult_expn del: subsetI)
-  subgoal premises prems for k res'
-  apply (rule prems(1)[THEN spec[where x=r], THEN spec[where x=res'],
-              simplified prems, simplified, THEN mp])
-    apply (rule exI[where x=\<open>c * FIC_brk_frame.mk (1(k \<mapsto> nonsepable None))\<close>])
-  apply (simp add: \<phi>expns prems)
-  by (smt (verit, best) FIC_brk_frame.expand FIC_brk_frame.sep_disj_fiction Fic_Space_Un Fic_Space_m \<phi>Res_Spec_mult_homo prems(3) prems(4) prems(5) prems(6) prems(7) sep_disj_multD2 sep_disj_multI2 sep_mult_assoc)
-  by meson .
+  unfolding Brk_Frame_eq_identity
+  by (rule; simp add: finite_map_freshness)
 
-lemma
+private lemma dispose_brk_scope:
+  \<open>\<^bold>p\<^bold>r\<^bold>o\<^bold>c R_brk_frame.\<phi>R_set_res (\<lambda>f. f(l := None)) \<lbrace> Brk_Frame l \<longmapsto> \<lambda>_. Void \<rbrace>\<close>
+  unfolding Brk_Frame_eq_identity
+  by (rule FIC_brk_frame.\<phi>R_dispose_res[where P=\<open>\<lambda>_. True\<close>]; simp)
+
+lemma brk_scope:
   \<open> (\<And>l. \<^bold>p\<^bold>r\<^bold>o\<^bold>c f l \<lbrace> X\<heavy_comma> Brk_Frame l \<longmapsto> \<lambda>ret. Y ret\<heavy_comma> Brk_Frame l \<rbrace>
-    \<^bold>t\<^bold>h\<^bold>r\<^bold>o\<^bold>w\<^bold>s (\<lambda>a. (E1 a\<heavy_comma> y \<Ztypecolon> Brking_Frame l U) + (E2 a\<heavy_comma> Brk_Frame l)))
-\<Longrightarrow> \<^bold>p\<^bold>r\<^bold>o\<^bold>c op_brk_scope f \<lbrace> X \<longmapsto> \<lambda>ret. Y ret + S ret \<rbrace> \<^bold>t\<^bold>h\<^bold>r\<^bold>o\<^bold>w\<^bold>s E2\<close>
+    \<^bold>t\<^bold>h\<^bold>r\<^bold>o\<^bold>w\<^bold>s (\<lambda>a. (Brking_Frame l Y') + (E a\<heavy_comma> Brk_Frame l)))
+\<Longrightarrow> \<^bold>p\<^bold>r\<^bold>o\<^bold>c op_brk_scope f \<lbrace> X \<longmapsto> \<lambda>ret. Y ret + Y' ret \<rbrace> \<^bold>t\<^bold>h\<^bold>r\<^bold>o\<^bold>w\<^bold>s E\<close>
   unfolding op_brk_scope_def
-  apply (rule alloc, rule "__op_try__", rule, assumption, rule)
-  thm "__op_try__"
-  thm R_brk_frame.\<phi>R_allocate_res_entry
+  apply (rule, rule, rule, assumption, rule)
+  apply (rule \<phi>CONSEQ'E0, rule dispose_brk_scope[THEN \<phi>frame, simplified], rule)
+  apply (rule \<phi>CASE)
+  apply (simp only: Brking_Frame_eq_identity norm_precond_ex, rule, rule, simp, rule)
+  apply (rule FIC_brk_frame.\<phi>R_dispose_res_frm[where P=\<open>\<lambda>_. True\<close>]; simp)
+  apply (rule)
+  apply (simp only: Brk_Frame_eq_identity, rule, simp, rule)
+   apply (rule \<phi>CONSEQ'E0, rule FIC_brk_frame.\<phi>R_dispose_res_frm[where P=\<open>\<lambda>_. True\<close>]; simp)
+  by (rule, rule implies_refl)
+
+lemma op_break_\<phi>app:
+  \<open>\<^bold>p\<^bold>r\<^bold>o\<^bold>c op_break l vs \<lbrace> S vs\<heavy_comma> Brk_Frame l \<longmapsto> (0 :: unreachable sem \<Rightarrow> _) \<rbrace>
+   \<^bold>t\<^bold>h\<^bold>r\<^bold>o\<^bold>w\<^bold>s (\<lambda>_. Brking_Frame l S)\<close>
+  unfolding op_break_def Brking_Frame_eq_identity Brk_Frame_eq_identity
+  by (rule, rule, simp, simp, simp, rule, \<phi>reason)
+
+end
 
 
-term \<open>
- op_try (F magic) (\<lambda>a.
-    if sem.dest a \<in> ABN_break.domain \<and> fst (ABN_break.dest (sem.dest a)) = magic
-    then Return (sem (from_vals (snd (ABN_break.dest (sem.dest a)))))
-    else det_lift (Exception a))\<close>
 
-definition \<phi>Break :: \<open>cf_label \<Rightarrow> ('vs::VALs sem \<Rightarrow> assn) \<Rightarrow> ABNM sem \<Rightarrow> assn\<close>
-  where \<open>\<phi>Break l S = (\<lambda>a. (S vs \<^bold>s\<^bold>u\<^bold>b\<^bold>j vs. ABN_break.mk (l, to_vals (sem.dest vs)) = sem.dest a))\<close>
+definition \<open>sift_brking_frame' l Y E = (Brking_Frame l Y) + (E\<heavy_comma> Brk_Frame l)\<close>
+definition \<open>sift_brking_frame = sift_brking_frame'\<close>
 
-term \<open>X \<^bold>i\<^bold>m\<^bold>p\<^bold>l\<^bold>i\<^bold>e\<^bold>s  \<close>
+lemma Brking_Frame_plus:
+  \<open>Brking_Frame l (Y1 + Y2) = Brking_Frame l Y1 + Brking_Frame l Y2\<close>
+  unfolding set_eq_iff Brking_Frame_def plus_fun_def distrib_right ExSet_plus by clarify
 
 lemma
-  \<open> (\<And>l. \<^bold>p\<^bold>r\<^bold>o\<^bold>c f l \<lbrace> X \<longmapsto> Y \<rbrace> \<^bold>t\<^bold>h\<^bold>r\<^bold>o\<^bold>w\<^bold>s (\<lambda>a. \<phi>Break l S a + E2 a))
-\<Longrightarrow> \<^bold>p\<^bold>r\<^bold>o\<^bold>c scope f \<lbrace> X \<longmapsto> \<lambda>ret. Y ret + S ret \<rbrace> \<^bold>t\<^bold>h\<^bold>r\<^bold>o\<^bold>w\<^bold>s E2\<close>
-  unfolding scope_def
-  apply (rule "__op_try__")
-   apply assumption
-  subgoal for ret
-    apply (cases ret)
-    apply (cases \<open>sem.dest ret \<in> ABN_break.domain \<and> fst (ABN_break.dest (sem.dest ret)) = magic\<close>; simp)
-prefer 2
-  unfolding \<phi>Break_def ABN_break.domain_def apply clarsimp
-  
-
-  unfolding \<phi>Procedure_def \<phi>Procedure_def
-  apply clarsimp apply rule
-  apply clarsimp
-subgoal for ret comp R x s
-    apply (cases s; simp; cases x; clarsimp simp add: \<phi>expns ring_distribs)
+  \<open> X1 \<^bold>i\<^bold>m\<^bold>p\<^bold>l\<^bold>i\<^bold>e\<^bold>s sift_brking_frame' l Y1 E1
+\<Longrightarrow> X2 \<^bold>i\<^bold>m\<^bold>p\<^bold>l\<^bold>i\<^bold>e\<^bold>s sift_brking_frame' l Y2 E2
+\<Longrightarrow> (X1 + X2) \<^bold>i\<^bold>m\<^bold>p\<^bold>l\<^bold>i\<^bold>e\<^bold>s sift_brking_frame' l (Y1 + Y2) (E1 + E2)\<close>
+  unfolding sift_brking_frame'_def Brking_Frame_plus distrib_right
+  \<medium_left_bracket> ;; ;; cases'
+  apply (clarsimp simp add: \<phi>expns Brking_Frame_plus)
 
 
-  unfolding scope_def op_try_def
-  apply clarsimp
-  unfolding \<phi>Procedure_def
-  apply clarsimp
-subgoal for comp R x s
-    apply (cases s; simp; cases x; clarsimp simp add: \<phi>expns ring_distribs)
-subgoal premises prems for a b u v
-      using prems(1)[THEN spec[where x=comp], THEN spec[where x=R]]
-      by (smt (verit) INTERP_SPEC LooseStateTy_expn(1) LooseStateTy_plus in_mono prems(2) prems(5) prems(6) prems(7) prems(8) set_mult_expn)
+hide_fact Brking_Frame_plus
 
+
+  notepad
+begin
+  define xx where \<open>xx \<equiv> 10\<close>
+  term xx
 end
